Add SemihashMap interface, rename proof commands to goal commands, allow deletion

Pantograph/SemihashMap.lean
@@ -18,7 +18,56 @@ structure Imp (β: Type u) where
 
 namespace Imp
 
+structure WF (m: Imp β): Prop where
+  capacity: m.data.size = m.deallocs.size
+  front_dealloc: ∀ i: Fin m.deallocs.size, (i < m.allocFront) → (m.deallocs.get i) < m.allocFront
+  front_data: ∀ i: Fin m.data.size, (i ≥ m.allocFront) → (m.data.get i).isNone
 
+def empty (capacity := 16): Imp β :=
+  {
+    data := mkArray capacity .none,
+    size := 0,
+    allocFront := 0,
+    deallocs := mkArray capacity 0,
+    lastDealloc := 0,
+  }
+
+private theorem list_get_replicate (x: α) (i: Fin (List.replicate n x).length):
+    List.get (List.replicate n x) i = x := by
+  sorry
+
+theorem empty_wf : WF (empty n: Imp β) := by
+  unfold empty
+  apply WF.mk
+  case capacity =>
+    conv =>
+      lhs
+      congr
+      simp
+    conv =>
+      rhs
+      congr
+      simp
+    simp
+  case front_dealloc =>
+    simp_all
+    intro i
+    intro a
+    contradiction
+  case front_data =>
+    simp_all
+    intro i
+    unfold Imp.data at i
+    simp at i
+    conv =>
+      lhs
+      unfold Array.get
+      unfold mkArray
+      simp [List.replicate]
+      rewrite [list_get_replicate]
+
+-- FIXME: Merge this with the well-formed versions below so proof and code can
+-- mesh seamlessly.
 @[inline] def insert (map: Imp β) (v: β): (Imp β × Nat) :=
   match map.lastDealloc with
   | 0 => -- Capacity is full, buffer expansion is required
@@ -53,8 +102,9 @@ namespace Imp
     }
     (result, nextIndex)
 
-@[inline] def remove (map: Imp β) (index: Nat): Imp β :=
-  match map.data.getD index .none with
+@[inline] def remove (map: Imp β) (index: Fin (map.size)): Imp β :=
+  have h: index.val < map.data.size := by sorry
+  match map.data.get ⟨index.val, h⟩ with
   | .none => map
   | .some _ =>
     {
@@ -66,24 +116,34 @@ namespace Imp
     }
 
 /-- Retrieval is efficient -/
-@[inline] def get? (map: Imp β) (index: Nat): Option β :=
-  map.data.getD index .none
+@[inline] def get? (map: Imp β) (index: Fin (map.size)): Option β :=
+  have h: index.val < map.data.size := by sorry
+  map.data.get ⟨index.val, h⟩
 @[inline] def capacity (map: Imp β): Nat := map.data.size
 
 end Imp
 
-def empty (capacity := 16): Imp β :=
-  {
-    data := mkArray capacity .none,
-    size := 0,
-    allocFront := 0,
-    deallocs := mkArray capacity 0,
-    lastDealloc := 0,
-  }
 
 /--
 This is like a hashmap but you cannot control the keys.
 -/
-def _root_.Pantograph.SemihashMap β := Imp β
+def _root_.Pantograph.SemihashMap β := {m: Imp β // m.WF}
+
+@[inline] def empty (capacity := 16): SemihashMap β :=
+  ⟨ Imp.empty capacity, Imp.empty_wf ⟩
+@[inline] def insert (map: SemihashMap β) (v: β): (SemihashMap β × Nat) :=
+  let ⟨imp, pre⟩ := map
+  let ⟨result, id⟩ := imp.insert v
+  ( ⟨ result, sorry ⟩, id)
+@[inline] def remove (map: SemihashMap β) (index: Nat): SemihashMap β :=
+  let ⟨imp, pre⟩ := map
+  let result := imp.remove ⟨index, sorry⟩
+  ⟨ result, sorry ⟩
+@[inline] def get? (map: SemihashMap β) (index: Nat): Option β :=
+  let ⟨imp, _⟩ := map
+  imp.get? ⟨index, sorry⟩
+@[inline] def size (map: SemihashMap β): Nat :=
+  let ⟨imp, _⟩ := map
+  imp.size
 
 end Pantograph.SemihashMap
